\section{Reihenentwicklungen}
\begin{alignat}{4}
&\sum\limits_{k=0}^{n}{\frac{1}{k!}}&&= 1+\frac{1}{1!}+\frac{1}{2!}+\frac{1}{3!}\ldots+\frac{1}{n!} \quad&&\overset{n\rightarrow\infty}{\longrightarrow}\quad \e\nonumber\\[0.1cm]
&\sum\limits_{k=0}^{n}{(-1)^{k}\frac{1}{k!}}&&= 1-\frac{1}{1!}+\frac{1}{2!}-\frac{1}{3!}+\ldots\pm\frac{1}{n!}\qquad&&\overset{n\rightarrow\infty}{\longrightarrow}\quad  \frac1\e\nonumber\\[0.0cm]
&\sum\limits_{k=0}^{n}{(-1)^{k}\frac{1}{k}}&&= 1-\frac{1}{2}+\frac{1}{3}-\frac{1}{4}+\ldots\pm\frac{1}{n}\qquad&&\overset{n\rightarrow\infty}{\longrightarrow}\quad \ln (2)\nonumber\\[0.0cm]
&\sum\limits_{k=0}^{n}{\frac{1}{2^k}}&&= 1+\frac{1}{2^1}+\frac{1}{2^2}-\frac{1}{2^3}+\ldots+\frac{1}{2^n}\qquad&&\overset{n\rightarrow\infty}{\longrightarrow}\quad 2\nonumber\\[0.0cm]
%&\sum\limits_{k=0}^{n}{(-1)^{k}\frac{1}{2^k}}&&= 1-\frac{1}{2^1}+\frac{1}{2^2}-\frac{1}{2^3}+\ldots\pm\frac{1}{2^n}\qquad&&\overset{n\rightarrow\infty}{\longrightarrow}\quad  \frac23\nonumber\\[0.0cm]
&\sum\limits_{k=0}^{n}{\frac{1}{k(k+1)}}&&= \frac{1}{1\cdot2}+\frac{1}{2\cdot3}+\frac{1}{3\cdot4}+\ldots+\frac{1}{n(n+1)}\qquad&&\overset{n\rightarrow\infty}{\longrightarrow}\quad 1\nonumber\\[0.0cm]
&\sum\limits_{k=0}^{n}{\frac{1}{(2k-1)(2k+1)}}&&= \frac{1}{1\cdot3}+\frac{1}{3\cdot5}+\frac{1}{5\cdot7}+\ldots+\frac{1}{(2n-1)(2n+1)}\qquad&&\overset{n\rightarrow\infty}{\longrightarrow}\quad \frac 12\nonumber\\[0.0cm]
&\sum\limits_{k=0}^{n}{\frac{1}{(k-1)(k+1)}}&&= \frac{1}{1\cdot3}+\frac{1}{2\cdot4}+\frac{1}{3\cdot5}+\ldots+\frac{1}{(n-1)(n+1)}\qquad&&\overset{n\rightarrow\infty}{\longrightarrow}\quad \frac 34\nonumber\\[0.0cm]
&\sum\limits_{k=0}^{n}{\frac{1}{k(k+1)(k+2)}}&&= \frac{1}{1\cdot2\cdot3}+\frac{1}{2\cdot3\cdot4}+\ldots+\frac{1}{n(n+1)(n+2)}\qquad&&\overset{n\rightarrow\infty}{\longrightarrow}\quad \frac 14\nonumber\\[0.0cm]
&\sum\limits_{k=0}^{n}{q^k}&&= q+q^2+q^3+\ldots+q^n\qquad&&\overset{n\rightarrow\infty}{\longrightarrow}\quad \frac{1}{1-q}\qquad&& 0\leq q<1\nonumber\\[0.0cm]
&\sum\limits_{k=1}^{n}{q^k}&&= q^2+q^3+q^4\ldots+q^n\qquad&&\overset{n\rightarrow\infty}{\longrightarrow}\quad  \frac{1}{1-q}-1\qquad&& 0\leq q<1\nonumber\\[0.0cm]
&\sum\limits_{k=0}^{n}{\binom{\alpha}{k}x^k}&&\qquad&&\overset{n\rightarrow\infty}{\longrightarrow}\quad  (1+x)^\alpha\qquad&& 0\leq x<1\nonumber\\
&\sum\limits_{k=0}^{n}{k\alpha^k}&&=\alpha+ 2\alpha^2+3\alpha^3\qquad+\ldots+n\alpha^n&&\overset{n\rightarrow\infty}{\longrightarrow}\quad  \frac{\alpha}{\left(1-\alpha\right)^2}\qquad&& 0\leq \alpha<1\nonumber
\end{alignat}

\vfill
